
@prefix adr:  <http://kg.artsdata.ca/resource/> .
@prefix ado:  <http://kg.artsdata.ca/ontology/> .
@prefix owl: <http://www.w3.org/2002/07/owl#> .
@prefix rdf: <http://www.w3.org/1999/02/22-rdf-syntax-ns#> .
@prefix xml: <http://www.w3.org/XML/1998/namespace> .
@prefix xsd: <http://www.w3.org/2001/XMLSchema#> .
@prefix rdfs: <http://www.w3.org/2000/01/rdf-schema#> .
@prefix skos: <http://www.w3.org/2004/02/skos/core#> .
@prefix dcterms: <http://purl.org/dc/terms/> .
@prefix vann: <http://purl.org/vocab/vann/> .
@prefix schema:  <http://schema.org/> .

ado: rdf:type owl:Ontology ;
    dcterms:title "Artsdata Ontology"@en ;
    dcterms:description "The Artsdata Ontology is designed to model and represent data related to arts, culture, and heritage."@en ;
    dcterms:creator "Artsdata Stewardship Team" ;
    dcterms:created "2025-09-30"^^xsd:date ;
    dcterms:modified "2025-10-17"^^xsd:date ;
    dcterms:license <http://creativecommons.org/licenses/by/4.0/> ;
    vann:preferredNamespacePrefix "ado" ;
    vann:preferredNamespaceUri "http://kg.artsdata.ca/ontology/" ;
    owl:versionIRI <http://kg.artsdata.ca/ontology/1/> ; # TODO: location = /ontology/1 { return 301 /ontology/; }
    owl:versionInfo "1.0.0" ;
    dcterms:hasFormat <https://raw.githubusercontent.com/culturecreates/artsdata-data-model/refs/heads/master/ontology/artsdata-ontology.ttl> .

####################
# Classes
####################
ado:Thing rdf:type rdfs:Class ; 
    rdfs:label "Thing"@en ;
    rdfs:comment "The most generic class of things in Artsdata."@en ;
    rdfs:isDefinedBy ado: .

ado:LivePerformanceWork rdf:type rdfs:Class ;
    rdfs:label "Live Performance Work"@en,  "Œuvre scénique"@fr;
    rdfs:comment "A work that is performed live, such as a play, concert, or dance performance."@en ;
    rdfs:isDefinedBy ado: ;
    rdfs:subClassOf ado:Thing ;
    schema:alternateName "show"@en, "spectacle"@fr .

ado:EventType rdf:type rdfs:Class ;
    rdfs:label "Event Type"@en ;
    rdfs:comment "A class representing different types of events."@en ;
    rdfs:isDefinedBy ado: ;
    rdfs:subClassOf skos:Concept, ado:Thing .

ado:Genre rdf:type rdfs:Class ;
    rdfs:label "Genre"@en ;
    rdfs:comment "A class representing different genres of artistic works."@en ;
    rdfs:isDefinedBy ado: ;
    rdfs:subClassOf skos:Concept, ado:Thing .

ado:Event rdf:type rdfs:Class ;
    rdfs:label "Event"@en ;
    rdfs:comment "An event is a happening that occurs at a certain time and location. Examples include and are not limited to a: performance, concert, conference, festival, exhibition and/or social gathering."@en ;
    owl:equivalentClass schema:Event, ado:Thing ;
    rdfs:isDefinedBy ado: ;
    schema:alternateName "performance"@en, "représentation"@fr .

####################
# Properties
####################

ado:hasEventType rdf:type rdf:Property ;
    rdfs:label "has event type"@en ;
    rdfs:comment "Links an Event to an event type defined by the Artsdata controlled vocabulary for event types."@en ;
    rdfs:isDefinedBy ado: ;
    rdfs:domain ado:Event ;
    rdfs:range ado:EventType .

ado:hasGenre rdf:type rdf:Property ;
    rdfs:label "has genre"@en ;
    rdfs:comment "Links a Live Performance Work to a genre defined by the Artsdata controlled vocabulary for genres."@en ;
    rdfs:isDefinedBy ado: ;
    rdfs:domain ado:LivePerformanceWork ;
    rdfs:range ado:Genre .